flake.nix
@@ -1,7 +1,7 @@
 {
   inputs = {
-    flake-utils.url = github:numtide/flake-utils;
-    nixpkgs.url = github:NixOS/nixpkgs/nixos-unstable;
+    flake-utils.url = "github:numtide/flake-utils";
+    nixpkgs.url = "github:NixOS/nixpkgs/nixos-unstable";
   };
 
   outputs = {nixpkgs, flake-utils, ...}:
@@ -10,30 +10,20 @@
     in flake-utils.lib.eachSystem systems (system:
       let
         pkgs = import nixpkgs { inherit system; };
-        self_pkgs = pkgs.callPackage ./nix/packages.nix {};
+        self_pkgs = pkgs.callPackage ./nix/packages.nix {
+          coqPackages=pkgs.coqPackages_8_16;
+        };
         python3 = pkgs.python3;
       in
       rec {
         packages = with self_pkgs; {
           catala = coqPackages.catala;
-          catala_8_5 = coqPackages_8_5.catala;
-          catala_8_6 = coqPackages_8_6.catala;
-          catala_8_7 = coqPackages_8_7.catala;
-          catala_8_8 = coqPackages_8_8.catala;
-          catala_8_9 = coqPackages_8_9.catala;
-          catala_8_10 = coqPackages_8_10.catala;
-          catala_8_11 = coqPackages_8_11.catala;
-          catala_8_12 = coqPackages_8_12.catala;
-          catala_8_13 = coqPackages_8_13.catala;
-          catala_8_14 = coqPackages_8_14.catala;
-          catala_8_15 = coqPackages_8_15.catala;
-          catala_8_16 = coqPackages_8_16.catala;
           default = coqPackages.catala;
         };
         devShell = pkgs.mkShell {
           inputsFrom = [ packages.catala ];
           buildInputs = [
-            pkgs.coqPackages.serapi
+            self_pkgs.coqPackages.serapi
             python3.pkgs.alectryon
             python3.pkgs.rich
           ];
