nix/packages.nix
@@ -1,29 +1,5 @@
-{ coqPackages
-, coqPackages_8_5
-, coqPackages_8_6
-, coqPackages_8_7
-, coqPackages_8_8
-, coqPackages_8_9
-, coqPackages_8_10
-, coqPackages_8_11
-, coqPackages_8_12
-, coqPackages_8_13
-, coqPackages_8_14
-, coqPackages_8_15
-, coqPackages_8_16 }:
+{ coqPackages }:
 
 {
-  coqPackages_8_5 = coqPackages_8_5.overrideScope' (self: super: {catala=self.callPackage ./catala.nix {};});
-  coqPackages_8_6 = coqPackages_8_6.overrideScope' (self: super: {catala=self.callPackage ./catala.nix {};});
-  coqPackages_8_7 = coqPackages_8_7.overrideScope' (self: super: {catala=self.callPackage ./catala.nix {};});
-  coqPackages_8_8 = coqPackages_8_8.overrideScope' (self: super: {catala=self.callPackage ./catala.nix {};});
-  coqPackages_8_9 = coqPackages_8_9.overrideScope' (self: super: {catala=self.callPackage ./catala.nix {};});
-  coqPackages_8_10 = coqPackages_8_10.overrideScope' (self: super: {catala=self.callPackage ./catala.nix {};});
-  coqPackages_8_11 = coqPackages_8_11.overrideScope' (self: super: {catala=self.callPackage ./catala.nix {};});
-  coqPackages_8_12 = coqPackages_8_12.overrideScope' (self: super: {catala=self.callPackage ./catala.nix {};});
-  coqPackages_8_13 = coqPackages_8_13.overrideScope' (self: super: {catala=self.callPackage ./catala.nix {};});
-  coqPackages_8_14 = coqPackages_8_14.overrideScope' (self: super: {catala=self.callPackage ./catala.nix {};});
-  coqPackages_8_15 = coqPackages_8_15.overrideScope' (self: super: {catala=self.callPackage ./catala.nix {};});
-  coqPackages_8_16 = coqPackages_8_16.overrideScope' (self: super: {catala=self.callPackage ./catala.nix {};});
   coqPackages = coqPackages.overrideScope' (self: super: {catala=self.callPackage ./catala.nix {};});
 }
